aux.v
@@ -1,0 +1,172 @@
+Require Import ZArith String Ascii NZAxioms.
+
+(* Auxiliary. *)
+
+Ltac magic := intros; auto; try easy; try intuition; simpl.
+
+Ltac black_magic := intros; auto; try easy; try intuition; try zify; try omega; simpl.
+
+Ltac magics := repeat black_magic.
+
+Local Open Scope N_scope.
+
+Definition byte_range_size := 256.
+
+Definition two_bytes_range_size := 65536.
+
+Definition ascii_to_string (c : ascii) : string := String c EmptyString.
+
+Definition two_ascii_to_string (c1 : ascii) (c2 : ascii) : string :=
+  String c1 (String c2 EmptyString).
+
+(* Convert a number in the range 0 <= n < 65536 to a two-char string. *)
+Definition word_no_to_string (word_no : N) : string := two_ascii_to_string 
+  (ascii_of_N (word_no / byte_range_size)) 
+  (ascii_of_N (word_no mod byte_range_size)).
+
+(* Convert a number in the range 0 <= n < 65536 encoded in a two-char string to N. *)
+Definition string_to_word_no (s: string) : option N :=
+  match s with
+  | String c1 (String c2 EmptyString) => Some (N_of_ascii c1 * byte_range_size + N_of_ascii c2)
+  | _ => None
+  end.
+
+Lemma char_less_than_256 : forall c, N_of_ascii c < byte_range_size.
+Proof.
+intros.
+destruct c.
+destruct b;
+destruct b0;
+destruct b1;
+destruct b2;
+destruct b3;
+destruct b4;
+destruct b5;
+destruct b6;
+easy.
+Qed.
+
+Theorem string_to_word_no_in_range : forall s x, 
+  string_to_word_no s = Some x -> x < two_bytes_range_size.
+Proof.
+unfold string_to_word_no.
+simpl.
+intros s x.
+destruct s; auto.
+* intros.
+  exfalso.
+  inversion H.
+* destruct s; auto.
+  + intros.
+    exfalso.
+    inversion H.
+  + destruct s; auto.
+    Focus 2.
+    - intro.
+      exfalso.
+      inversion H.
+assert (N_of_ascii a < byte_range_size) as aLower.
+{ apply (char_less_than_256 a). }
+
+assert (N_of_ascii a0 < byte_range_size) as a0Lower.
+{ apply (char_less_than_256 a0). }
+intro.
+assert (N_of_ascii a * byte_range_size + N_of_ascii a0 = x) as Rew.
+{ inversion H. 
+  auto. }
+rewrite <- Rew.
+clear Rew.
+clear H.
+clear x.
+destruct (N_of_ascii a); destruct (N_of_ascii a0); auto.
+- assert (0 * byte_range_size + N.pos p = N.pos p).
+  { easy. }
+  rewrite H.
+  assert (byte_range_size < two_bytes_range_size).
+  { easy. }
+  rewrite a0Lower.
+  assumption.
+- rewrite (N.add_0_r (N.pos p * byte_range_size)).
+  assert (byte_range_size * byte_range_size = two_bytes_range_size).
+  { easy. }
+  rewrite <- H.
+  rewrite <- (N.mul_lt_mono_pos_r byte_range_size (N.pos p) byte_range_size).
+  -- assumption.
+  -- easy.
+- assert (N.pos p * byte_range_size <= (byte_range_size - 1) * byte_range_size).
+  { magics. }
+  magic.
+  unfold two_bytes_range_size.
+  Local Close Scope N_scope.
+  Local Open Scope positive_scope.
+  cut (p * 256 + p0 < 65536).
+  { magics. }
+  unfold byte_range_size in H.
+  unfold byte_range_size in aLower.
+  unfold byte_range_size in a0Lower.
+  simpl in H.
+  magics.
+Qed.
+
+
+Local Close Scope positive_scope.
+Local Open Scope N_scope.
+
+Lemma div_mul_mod_ident : forall x y, y <> 0 -> x / y * y + x mod y = x.
+Proof.
+intros.
+rewrite (N.mul_comm (x / y) y).
+rewrite <- (N.div_mod x y).
+all: auto.
+Qed.
+
+Theorem word_no_string_ident : forall word_no, 
+  word_no < two_bytes_range_size -> 
+  Some word_no = string_to_word_no (word_no_to_string word_no).
+Proof.
+intros.
+simpl.
+
+assert (word_no < byte_range_size * byte_range_size).
+{ easy. }
+
+assert (word_no / byte_range_size < byte_range_size) as UpperIneq.
+{ apply N.div_lt_upper_bound; auto.
+  easy. }
+
+assert (word_no mod byte_range_size < byte_range_size) as LowerIneq.
+{ apply N.mod_bound_pos.
+  * destruct word_no; easy.
+  * easy. }
+
+rewrite (N_ascii_embedding (word_no / byte_range_size)).
+* rewrite (N_ascii_embedding (word_no mod byte_range_size)).
+  + rewrite (div_mul_mod_ident word_no byte_range_size).
+    - auto.
+    - easy.
+  + easy.
+* easy.
+Qed.
+
+
+Local Close Scope N_scope.
+Local Open Scope positive_scope.
+
+Definition null_terminate (s : string) : string :=
+  s ++ String zero EmptyString.
+
+Fixpoint str_last (s : string) : ascii :=
+  match s with
+  | EmptyString => zero
+  | String c EmptyString => c
+  | String _ rest => str_last rest
+  end.
+
+Theorem last_null : forall s, str_last (null_terminate s) = zero.
+Proof with magics.
+magics.
+unfold null_terminate...
+unfold str_last...
+elim s...
+destruct s0...
+Qed.
