errcode.v
@@ -1,0 +1,61 @@
+(* Error codes. *)
+
+Inductive error_code : Set := 
+| NOT_DEFINED 
+| FILE_NOT_FOUND 
+| ACCESS_VIOLATION
+| DISK_FULL_OR_ALLOCATION_EXCEEDED
+| ILLEGAL_TFTP_OPERATION
+| UNKNOWN_TRANSFER_ID
+| FILE_ALREADY_EXISTS
+| NO_SUCH_USER.
+
+Definition err_code_to_nr (err : error_code) : N := 
+  match err with 
+  | NOT_DEFINED => 0
+  | FILE_NOT_FOUND => 1
+  | ACCESS_VIOLATION => 2
+  | DISK_FULL_OR_ALLOCATION_EXCEEDED => 3
+  | ILLEGAL_TFTP_OPERATION => 4
+  | UNKNOWN_TRANSFER_ID => 5
+  | FILE_ALREADY_EXISTS => 6
+  | NO_SUCH_USER => 7
+  end.
+
+Definition nr_to_err_code (nr : N) : option error_code :=
+  match nr with
+  | N0 => Some NOT_DEFINED
+  | Npos 1 => Some FILE_NOT_FOUND 
+  | Npos 2 => Some ACCESS_VIOLATION
+  | Npos 3 => Some DISK_FULL_OR_ALLOCATION_EXCEEDED
+  | Npos 4 => Some ILLEGAL_TFTP_OPERATION
+  | Npos 5 => Some UNKNOWN_TRANSFER_ID
+  | Npos 6 => Some FILE_ALREADY_EXISTS
+  | Npos 7 => Some NO_SUCH_USER
+  | _ => None
+  end.
+
+Theorem err_code_nr_ident : forall err, Some err = nr_to_err_code (err_code_to_nr err).
+Proof.
+intros.
+destruct err; simpl; auto.
+Qed.
+
+Definition err_code_to_string (err : error_code) : string :=
+  word_no_to_string (err_code_to_nr err).
+
+Definition string_to_err_code (s : string) : option error_code := 
+  string_to_word_no s >>= nr_to_err_code.
+
+Theorem err_code_string_ident : forall err, Some err = string_to_err_code (err_code_to_string err).
+Proof.
+intros.
+case err;
+unfold err_code_to_string;
+simpl;
+unfold word_no_to_string;
+simpl;
+unfold string_to_err_code;
+simpl;
+auto.
+Qed.
