maybe.v
@@ -1,0 +1,37 @@
+(* Maybe monad *)
+Arguments Some [A] _.
+Arguments None [A].
+
+Definition ret {A : Type} (x : A) := Some x.
+ 
+Definition bind {A B : Type} (a : option A) (f : A -> option B) : option B :=
+  match a with
+    | Some x => f x
+    | None => None
+  end.
+
+Notation "A >>= F" := (bind A F) (at level 42, left associativity).
+
+Notation "'do' X <- A ; B" := (bind A (fun X => B)) (at level 200, X ident, A at level 100, B at level 200).
+
+Lemma mon_left_id : forall (A B : Type) (a : A) (f : A -> option B),
+  ret a >>= f = f a.
+Proof.
+intros.
+reflexivity.
+Qed.
+ 
+Lemma mon_right_id : forall (A : Type) (a : option A),
+  a >>= ret = a.
+Proof.
+intros.
+induction a; repeat reflexivity.
+Qed.
+ 
+Lemma mon_assoc :
+  forall (A B C : Type) (a : option A) (f : A -> option B) (g : B -> option C),
+    (a >>= f) >>= g = a >>= (fun x => f x >>= g).
+Proof.
+intros.
+induction a; repeat reflexivity.
+Qed.
