opcode.v
@@ -1,0 +1,93 @@
+Require Import String ZArith Ascii.
+
+(* Opcodes. *)
+
+Local Open Scope positive_scope.
+
+Inductive packet_opcode : Set := RRQ | WRQ | DATA | ACK | ERROR.
+
+Definition opcode_to_nr (code: packet_opcode) :=
+  match code with  
+  | RRQ   => 1
+  | WRQ   => 2
+  | DATA  => 3
+  | ACK   => 4
+  | ERROR => 5
+  end.
+
+Lemma opcode_range : forall x, 1 <= opcode_to_nr x <= 5.
+Proof.
+intros.
+destruct x.
+all: easy.
+Qed.
+
+
+Definition nr_to_opcode (nr: positive) : option packet_opcode := 
+  match nr with
+  | 1 => Some RRQ
+  | 2 => Some WRQ
+  | 3 => Some DATA
+  | 4 => Some ACK
+  | 5 => Some ERROR
+  | _ => None
+  end.
+
+Lemma nr_opcode_ident : forall x, x <= 5 ->
+  match nr_to_opcode x with 
+    | Some opcode => x = opcode_to_nr opcode
+    | None => True
+  end.
+Proof.
+intros x bound.
+unfold opcode_to_nr.
+destruct x; simpl.
+* destruct x; auto.
+  destruct x; auto.
+* destruct x; auto.
+  destruct x; auto.
+* auto.
+Qed.
+
+
+
+
+Lemma nr_opcode_none : forall x, x > 5 \/ x < 1 -> nr_to_opcode x = None.
+Proof.
+intros.
+unfold nr_to_opcode.
+case H.
+* intro gt5.
+  destruct x.
+  + destruct x; auto.
+    - destruct x; easy.
+    - easy.
+  + destruct x; auto.
+    - destruct x; easy.
+    - easy.
+  + easy.
+* intro.
+  destruct x.
+  all: easy.
+Qed.
+
+
+Definition opcode_to_ascii (op : packet_opcode) : ascii :=
+   ascii_of_pos (opcode_to_nr op).
+
+Definition ascii_to_opcode (c : ascii) : option packet_opcode :=
+  match N_of_ascii c with
+  | Npos p => nr_to_opcode p
+  | _ => None
+  end.
+
+Theorem opcode_ascii_ident : 
+  forall op : packet_opcode, 
+  Some op = ascii_to_opcode (opcode_to_ascii op).
+Proof.
+intros.
+destruct op; auto.
+Qed.
+
+Definition opcode_to_string (op : packet_opcode) : string := 
+  String zero (String (opcode_to_ascii op) EmptyString).
